src/lowparse/LowParse.Steel.Validate.fst
@@ -5,7 +5,6 @@ include LowParse.Low.ErrorCode
 module S = Steel.Memory
 module SE = Steel.Effect
 module SEA = Steel.Effect.Atomic
-module A = Steel.C.Array
 module AP = LowParse.Steel.ArrayPtr
 
 module SZ = Steel.C.StdInt.Base
@@ -68,7 +67,7 @@ let tvalidator
   SE.Steel bool
     (AP.varrayptr a)
     (tvalid_res_vprop p a)
-    (fun h -> U32.v len == A.length (h (AP.varrayptr a)).AP.array)
+    (fun h -> U32.v len == AP.length (h (AP.varrayptr a)).AP.array)
     (fun h res h' ->
       let s = h (AP.varrayptr a) in
       let s' = h' (tvalid_res_vprop p a res) in
@@ -104,7 +103,7 @@ let wvalidator
   SE.Steel U64.t
     (AP.varrayptr a)
     (fun _ -> AP.varrayptr a)
-    (fun h -> U32.v len == A.length (h (AP.varrayptr a)).AP.array)
+    (fun h -> U32.v len == AP.length (h (AP.varrayptr a)).AP.array)
     (fun h res h' ->
       let s = h (AP.varrayptr a) in
       h' (AP.varrayptr a) == s /\
@@ -137,13 +136,13 @@ let wvalidate_post // FIXME: WHY WHY WHY do I need to define this postcondition 
     s' == s
   else begin
     let s' : v base k t = s' in
-    let consumed = A.length (array_of s') in
+    let consumed = AP.length (array_of s') in
     Some? vres /\
-    U32.v len == A.length s.AP.array /\
+    U32.v len == AP.length s.AP.array /\
 //    perm_of s' == s.AP.perm /\
 //    (Some?.v vres).AP.perm == s.AP.perm /\
-    A.merge_into (array_of s') (Some?.v vres).AP.array s.AP.array /\
-    consumed <= A.length s.AP.array /\
+    AP.merge_into (array_of s') (Some?.v vres).AP.array s.AP.array /\
+    consumed <= AP.length s.AP.array /\
     is_byte_repr p s'.contents (Seq.slice s.AP.contents 0 consumed) /\
     (Some?.v vres).AP.contents == Seq.slice s.AP.contents consumed (U32.v len)
   end
@@ -159,7 +158,7 @@ val wvalidate
 : SE.Steel (byte_array base)
     (AP.varrayptr a)
     (fun res -> (if AP.g_is_null res then AP.varrayptr a else vparse p a) `SE.star` AP.varrayptr_or_null res)
-    (fun h -> U32.v len == A.length (h (AP.varrayptr a)).AP.array)
+    (fun h -> U32.v len == AP.length (h (AP.varrayptr a)).AP.array)
     (fun h res h' ->
       let s = h (AP.varrayptr a) in
       let s'  = h' (if AP.g_is_null res then AP.varrayptr a else vparse p a) in
@@ -200,7 +199,7 @@ let dummy
 : SE.Steel unit
     (AP.varrayptr a)
     (fun _ -> AP.varrayptr a)
-    (fun h -> U32.v len == A.length (h (AP.varrayptr a)).AP.array)
+    (fun h -> U32.v len == AP.length (h (AP.varrayptr a)).AP.array)
     (fun h _ h' ->
       h' (AP.varrayptr a) == h (AP.varrayptr a)
     )
@@ -222,7 +221,7 @@ let dummy
     let g1 : Ghost.erased (v base k t) = SEA.gget (vparse p a) in // FIXME: WHY WHY WHY is this type annotation needed?
     elim_vparse p a;
     let g2 : Ghost.erased (AP.v base byte) = SEA.gget (AP.varrayptr a) in
-    let glen = Ghost.hide (A.length (array_of (Ghost.reveal g1))) in
+    let glen = Ghost.hide (AP.length (array_of (Ghost.reveal g1))) in
     is_byte_repr_injective p (Ghost.reveal g1).contents (Seq.slice (Ghost.reveal g0).AP.contents 0 (Ghost.reveal glen)) (Ghost.reveal g2).AP.contents;
     Seq.lemma_split (Ghost.reveal g0).AP.contents (Ghost.reveal glen);
     AP.join a res
